\documentclass{article}
\usepackage{epsfig}
\pagestyle{empty}
\begin{document}
$ M \times N $
\pagebreak

$\overline{\textbf{m}}$
\pagebreak

$ \left(\overline{\textbf{m}}\right)_{ij} = \overline{\textbf{m}_{ij}},\ \forall i,j $
\pagebreak

$\textbf{m}$
\pagebreak

$ \left(\textbf{m}}_{ij} = \mathbb{R}\{\textbf{m}_{ij}\},\ \forall i,j $
\pagebreak

$ \left(\textbf{m}}_{ij} = \mathbb{I}\{\textbf{m}_{ij}\},\ \forall i,j $
\pagebreak

$ N \times M $
\pagebreak

$ \textbf{m}^{\mathrm{T}} $
\pagebreak

$ \left(\textbf{m}^{\mathrm{T}}\right)_{ij} = \textbf{m}_{ji},\ \forall i,j $
\pagebreak

$ \textbf{m}^{*} $
\pagebreak

$ \left(\textbf{m}^{*}\right)_{ij} = \overline{\textbf{m}_{ji}},\ \forall i,j $
\pagebreak

$M \times N$
\pagebreak

$N \times P$
\pagebreak

$ M \times P $
\pagebreak

$ \textbf{a}\textbf{b} $
\pagebreak

$ \left(\textbf{ab}\right)_{ij} = \sum\limits_{k=1}^{N}\textbf{a}_{ik}\textbf{b}_{kj} $
\pagebreak

$P \times Q$
\pagebreak

$ MP \times NQ $
\pagebreak

$ \textbf{a}\otimes\textbf{b} $
\pagebreak

$ \left(\textbf{a}\otimes\textbf{b}\right)_{ij} = \textbf{a}_{\lfloor i/P \rfloor,\lfloor j/Q \rfloor}\textbf{b}_{i\textrm{%}P,j\textrm{%}Q} $
\pagebreak

$ i \textrm{%} P $
\pagebreak

$ i/P $
\pagebreak

$ {\left\lVert \textbf{m} \right\rVert}_1 $
\pagebreak

$ {\left\lVert \textbf{m} \right\rVert}_1 = \max\limits_j \sum\limits_{i=1}^M \left\lvert \textbf{m}_{ij} \right\rvert $
\pagebreak

$ {\left\lVert \textbf{m} \right\rVert}_\infty $
\pagebreak

$ {\left\lVert \textbf{m} \right\rVert}_\infty = \max\limits_i \sum\limits_{j=1}^N \left\lvert \textbf{m}_{ij} \right\rvert $
\pagebreak

$ \textbf{m} $
\pagebreak

$ \max\left(N, M\right) \cdot \epsilon \cdot {\left\lVert \textbf{m} \right\rVert}_\infty $
\pagebreak

$ \textrm{rank}\left(\textbf{m}\right) $
\pagebreak

$ M \times M $
\pagebreak

$ \left\lvert \textbf{m} \right\rvert $
\pagebreak

$ \textbf{m}^{-1}$
\pagebreak

$ \textbf{m}\textbf{m}^{-1} = \textbf{m}^{-1}\textbf{m} = \textbf{I}_{M} $
\pagebreak

$ \textrm{tr}\left(\textbf{m}\right) $
\pagebreak

$ \textrm{tr}\left(\textbf{m}\right) = \sum\limits_{n=1}^{M} \textbf{m}_{nn} $
\pagebreak

$ \textbf{a}_{ij} = \textbf{b}_{ij}\ \forall i,j \in 1\ .. N $
\pagebreak

$ \textbf{m} + a $
\pagebreak

$ \left(\textbf{m} + a\right)_{ij} = \textbf{m}_{ij} + a $
\pagebreak

$ a + \textbf{m} $
\pagebreak

$ \left(a + \textbf{m}\right)_{ij} = a + \textbf{m}_{ij} $
\pagebreak

$ \textbf{a} + \textbf{b} $
\pagebreak

$ \left(\textbf{a} + \textbf{b}\right)_{ij} = \textbf{a}_{ij} + \textbf{b}_{ij} $
\pagebreak

$ \textbf{m}a $
\pagebreak

$ \left(\textbf{m} a\right)_{ij} = \textbf{m}_{ij} a $
\pagebreak

$ a\textbf{m} $
\pagebreak

$ \left(a\textbf{m}\right)_{ij} = a\textbf{m}_{ij} $
\pagebreak

$ \textbf{a} \circ \textbf{b} $
\pagebreak

$ \left(\textbf{a} \circ \textbf{b}\right)_{ij} = \textbf{a}_{ij} \textbf{b}_{ij} $
\pagebreak

$ \textbf{m}/a $
\pagebreak

$ \left(\textbf{m}/a\right)_{ij} = \frac{\textbf{m}_{ij}}{a} $
\pagebreak

$ \textbf{a} \circ \textbf{b}' $
\pagebreak

$ {\textbf{b}_{ij}}' = \left(\textbf{b}_{ij}\right)^{-1}$
\pagebreak

$ \left(\textbf{a} \circ \textbf{b}'\right)_{ij} = \textbf{a}_{ij} {\textbf{b}'}_{ij} $
\pagebreak

$ f\left(\textbf{m}_{ij}, \ldots\right) $
\pagebreak

$ \textbf{M} $
\pagebreak

$ \textbf{m}_{ij} = f(i, j) $
\pagebreak

$ \textbf{m}_{ij} = \textrm{value}\ \forall i,j $
\pagebreak

$ I_N $
\pagebreak

$ \left(M\times\textrm{Row}\right) \times \left(N\times\textrm{Col}\right) $
\pagebreak

$ \textbf{m}' $
\pagebreak

$ \textbf{m}'_{ij} = \textbf{m}_{\left(i\ \textrm{mod}\ M\right),\ \left(j\ \textrm{mod}\ N \right)} $
\pagebreak

$ {\textbf{m}'}_{ij} = \begin{cases} \textbf{m}_{bj} & i = a\\ \textbf{m}_{aj} & i = b\\ \textbf{m}_{ij} & \textrm{otherwise} \end{cases} $
\pagebreak

$ {\textbf{m}'}_{ij} = \begin{cases} \textbf{m}_{ib} & j = a\\ \textbf{m}_{ia} & j = b\\ \textbf{m}_{ij} & \textrm{otherwise} \end{cases} $
\pagebreak

$ M \times \left(N+P\right) $
\pagebreak

$ \left[\textbf{a} \textbf{b}\right] $
\pagebreak

$ \left(\left[\textbf{a} \textbf{b}\right]\right)_{ij} = \begin{cases} \textbf{a}_{ij} & j < N\\ \textbf{b}_{i,\ \left(j - N\right)} & j \ge N \end{cases} $
\pagebreak

$ N \times P $
\pagebreak

$ \left(M+N\right) \times P $
\pagebreak

$ \left[\textbf{a}; \textbf{b}\right] $
\pagebreak

$ \left(\left[\textbf{a}; \textbf{b}\right]\right)_{ij} = \begin{cases} \textbf{a}_{ij} & i < M\\ \textbf{b}_{\left(i - M\right),\ j} & i \ge M \end{cases} $
\pagebreak

$ P \times Q $
\pagebreak

$ {\textbf{m}'}_{ij} = \textbf{m}_{\left(a + i\right),\ \left(b + j\right)} $
\pagebreak

$ N \times 1 $
\pagebreak

$ 1 \times N $
\pagebreak

$ \sqrt{x} $
\pagebreak

$ \lvert x \rvert $
\pagebreak

$ x^n $
\pagebreak

$n$
\pagebreak

$ \sqrt[\leftroot{-2}\uproot{2}n]{x} $
\pagebreak

$ \bar{x} $
\pagebreak

$ \overline{\textbf{v}} $
\pagebreak

$ \left(\overline{\textbf{v}}\right)_i = \overline{v_i} $
\pagebreak

$ \begin{bmatrix} \sqrt{v_1} & \ldots &\sqrt{v_N} \end{bmatrix} $
\pagebreak

$ \textbf{u} $
\pagebreak

$ \textbf{u}_i = \mathbb{R}\{\textbf{v}_i\} $
\pagebreak

$ \textbf{u}_i = \mathbb{I}\{\textbf{v}_i\} $
\pagebreak

$ \begin{bmatrix} \lvert v_1 \rvert & \ldots & \lvert v_N \rvert \end{bmatrix} $
\pagebreak

$ \textbf{a} \cdot \textbf{b} $
\pagebreak

$ \left(\textbf{a}\cdot\textbf{b}\right)_i = a_i \overline{b_i} $
\pagebreak

$ \sum\limits_{i} v_i $
\pagebreak

$ v_i $
\pagebreak

$ v_i \leq v_j,\ \forall j $
\pagebreak

$ v_i \geq v_j,\ \forall j $
\pagebreak

$ i $
\pagebreak

$ \textbf{a}_i = \textbf{b}_i\ \forall i \in 1\ .. N $
\pagebreak

$ \textbf{v} + a $
\pagebreak

$ \left(\textbf{v} + a\right)_i = \textbf{v}_i + a $
\pagebreak

$ a + \textbf{v} $
\pagebreak

$ \left(a + \textbf{v}\right)_i = a + \textbf{v}_i $
\pagebreak

$ \left(\textbf{a} + \textbf{b}\right)_i = \textbf{a}_i + \textbf{b}_i $
\pagebreak

$ \textbf{v}a $
\pagebreak

$ \left(\textbf{v}a\right)_i = \textbf{v}_i a $
\pagebreak

$ a\textbf{v} $
\pagebreak

$ \left(a\textbf{v}\right)_i = a\textbf{v}_i $
\pagebreak

$ \left(\textbf{a} \circ \textbf{b}\right)_i = \textbf{a}_i \textbf{b}_i $
\pagebreak

$ \textbf{v}/a $
\pagebreak

$ \left(\textbf{v}/a\right)_i = \frac{\textbf{v}_i}{a} $
\pagebreak

$ {\textbf{b}_i}' = \left(\textbf{b}_i\right)^{-1}$
\pagebreak

$ \left(\textbf{a} \circ \textbf{b}'\right)_i = \textbf{a}_i {\textbf{b}'}_i $
\pagebreak

$ f\left(\textbf{v}_i, \ldots\right) $
\pagebreak

$ f\left(f\left(\ldots f\left(\textrm{init}, \textbf{v}_1\right), \ldots\right), \textbf{v}_N \right) $
\pagebreak

$ \textbf{v} $
\pagebreak

$ \textbf{v}_i = \textrm{start} + i - 1 $
\pagebreak

$ \frac{\textbf{v}_N - \textbf{v}_1}{N-1} $
\pagebreak

$ \textbf{v}_i = \textrm{value}\ \forall i \in 1\ .. N$
\pagebreak

$ \textbf{v}_i = f(i) $
\pagebreak

$ \textbf{v} \gg n $
\pagebreak

$ \left(\textbf{v} \gg n\right)_i = \textbf{v}_{(i + n)\ \textrm{mod}\ N} $
\pagebreak

$ \textbf{v}_{\textrm{start}:\left(\textrm{start} + M - 1\right)} $
\pagebreak

$ \left(\textbf{v}_{\textrm{start}:\left(\textrm{start} + M - 1\right)}\right)_i = \textbf{v}_{\textrm{start} + i} $
\pagebreak

$ \left(\left[\textbf{a} \textbf{b}\right]\right)_i = \begin{cases} \textbf{a}_i & i < N\\ \textbf{b}_{i - N} & i \ge N \end{cases} $
\pagebreak

\end{document}
